\documentclass[12pt]{article}

\usepackage[utf8]{inputenc}
\usepackage[turkish]{babel}
\usepackage[T1]{fontenc}

\usepackage{amsmath}
\usepackage{amssymb}
\usepackage{amsthm}
\usepackage{geometry}
\usepackage{graphicx}

\begin{document}
    \shorthandoff{=}

    \section{Gauge-Invariance}
    Let 
    \begin{equation*}
        \dot{x}=Ax,\,y=Cx+b,\,\dot{b}=0
    \end{equation*}
    be given. The bias term is modeled as,
    \begin{equation*}
        b\triangleq \alpha C+\beta C^\perp
    \end{equation*}
    where $C^T C^\perp=(C^\perp)^T C=0$ or alternatively $C\perp C^\perp$,
    and the projection matrix is chosen as,
    \begin{equation*}
        \Pi\triangleq I-\frac{CC^T}{C^T C}
    \end{equation*}
    The following can be stated,
    \begin{equation*}
        \begin{split}
          \Pi C&=\left(I-\frac{CC^T}{C^T C}\right)C\\
          &=C-\frac{CC^T C}{C^T C}\\
          &=C-C\\
          \Pi C&=0
        \end{split}
    \end{equation*}
    and
    \begin{equation*}
        \begin{split}
          \Pi C^\perp&=\left(I-\frac{CC^T}{C^T C}\right)C^\perp\\
          &=C^\perp-\frac{CC^T C^\perp}{C^T C}\\
          \Pi C^\perp&=C^\perp
        \end{split}
    \end{equation*}
    The projection matrix applied on the bias $\Pi b$ gives,
    \begin{equation*}
        \begin{split}
          \Pi b&=\Pi (\alpha C+\beta C^\perp)\\
          &=\alpha \Pi C+\beta \Pi C^\perp\\
          &=\beta C^\perp
        \end{split}
    \end{equation*}
    $\Pi$ applied to the output gives,
    \begin{equation*}
        \begin{split}
            \Pi y&=\Pi (Cx+\alpha C+\beta C^\perp)\\
            &=\Pi Cx+\alpha \Pi C+\beta \Pi C^\perp\\
            &=\beta \Pi C^\perp\\
            &=\beta C^\perp
        \end{split}
    \end{equation*}
    and     
    $\beta$ can be recovered using,
    \begin{equation*}
        \begin{split}
            (C^\perp)^T(\Pi y&=\beta C^\perp)\\
            (C^\perp)^T\Pi y&=(C^\perp)^T\beta C^\perp\\
            (C^\perp)^T\Pi y&=\beta(C^\perp)^T C^\perp\\
            \beta&=\frac{(C^\perp)^T\Pi y}{(C^\perp)^T C^\perp}
        \end{split}
    \end{equation*}
    Here, the bias perpendicular to the output vector $C$ can be recovered but, the bias aligned with the output can not be recovered via the projection. This can also be observed by the following,
    \begin{equation*}
        \begin{split}  
            \dot{x}=Ax,\,y=Cx+b,\,\dot{b}=0\\
            \dot{x}=Ax,\,y=Cx+\alpha C+\beta C^\perp,\,\dot{\alpha C+\beta C^\perp}=0\\
            \dot{x}=Ax,\,y=C(x+\alpha)+\beta C^\perp,\,\dot{\alpha} C+\dot{\beta} C^\perp=0\\
            \dot{x}=Ax,\,y=C(x+\alpha)+\beta C^\perp,\,\dot{\alpha}=0,\,\dot{\beta}=0
        \end{split}
    \end{equation*}
    Defining $z\triangleq x+\alpha$,
    \begin{equation*}
        \begin{split}  
            \dot{z}=Az-\alpha A,\,y=Cz+\beta C^\perp ,\,\dot{\alpha}=0,\,\dot{\beta}=0
        \end{split}
    \end{equation*}
    gives
    \begin{equation*}
        \begin{split} 
            \begin{bmatrix}
                \dot{z}\\
                \dot{\alpha}
            \end{bmatrix}=
            \begin{bmatrix}
                A& -A\\
                0& 0
            \end{bmatrix}\begin{bmatrix}
                z\\
                \alpha
            \end{bmatrix},\,y=\begin{bmatrix}C& 0\end{bmatrix}
            \begin{bmatrix}
                z\\
                \alpha
            \end{bmatrix}+\beta C^\perp,\,x=\begin{bmatrix}I&-I\end{bmatrix}\begin{bmatrix}
                z\\
                \alpha
            \end{bmatrix}
        \end{split}
    \end{equation*}
    An observer as follows,
    \begin{equation*}
        \begin{bmatrix}
                \dot{\hat{z}}\\
                \dot{\hat{\alpha}}
            \end{bmatrix}=
            \begin{bmatrix}
                A& -A\\
                0& 0
            \end{bmatrix}\begin{bmatrix}
                \hat{z}\\
                \hat{\alpha}
            \end{bmatrix}+\begin{bmatrix}
            L\\L_\alpha
            \end{bmatrix}(y-\hat{y}),\,\hat{y}=\begin{bmatrix}C& 0\end{bmatrix}
            \begin{bmatrix}
                \hat{z}\\
                \hat{\alpha}
            \end{bmatrix}+\Pi y,\,\hat{x}=\begin{bmatrix}I&-I\end{bmatrix}\begin{bmatrix}
                \hat{z}\\
                \hat{\alpha}
            \end{bmatrix}
    \end{equation*}
    may be used to determine $x$ and $\alpha$ where $\beta$ is obtained using the projection.

\end{document}